libcrux-iot/sha3/proofs/aeneas-lean/LibcruxIotSha3/Sponge/XorBlockSpec.lean
@@ -63,7 +63,7 @@ open Aeneas Aeneas.Std Result Std.Do libcrux_iot_sha3 hacspec_sha3
 
 namespace libcrux_iot_sha3.Sponge
 
-open libcrux_iot_sha3.Equivalence
+open libcrux_iot_sha3.Foundation
 
 set_option allowUnsafeReducibility true in
 attribute [local irreducible] keccak.keccakf1600 keccak_f.keccak_f
